common/Var.v
@@ -5,12 +5,125 @@ From Coq Require Import FMaps FSets.
 From mathcomp Require Import ssreflect ssrbool ssrnat eqtype.
 From Common Require Import FMaps FSets Nats.
 
+Set Implicit Arguments.
+Unset Strict Implicit.
+Import Prenex Implicits.
+
+
+
 Definition var : Set := nat.
 
-Module VM := FMapList.Make(NatOrder).
+(* Variable sets. *)
 
-Module VMLemmas := FMapLemmas(VM).
+Module VS.
+  Module S := FSetList.Make(NatOrder).
+  Module Lemmas := FSetLemmas(S).
+  Include S.
 
-Module VS := FSetList.Make(NatOrder).
+  (* Generate a new variable. *)
+  Definition new_var (s : t) : var :=
+    match max_elt s with
+    | Some v => v + 1
+    | None => 0
+    end.
 
-Module VSLemmas := FSetLemmas(VS).
+  Lemma new_var_is_new :
+    forall (s : t), ~~ mem (new_var s) s.
+  Proof.
+    move=> s.
+    apply/negP => Hmem.
+    move: (mem_2 Hmem) => {Hmem}.
+    rewrite /new_var.
+    case H: (max_elt s).
+    - move=> Hin.
+      move: (max_elt_2 H Hin) => Hfalse.
+      apply: Hfalse.
+      rewrite addn1.
+      exact: ltnSn.
+    - move: (max_elt_3 H) => {H} H Hin.
+      move: (H 0) => Hnotin; apply: Hnotin; exact: Hin.
+  Qed.
+
+End VS.
+
+
+
+(* Variable maps. *)
+
+Module VM.
+   Module M := FMapList.Make(NatOrder).
+   Module Lemmas := FMapLemmas(M).
+   Include M.
+
+   Section Aux.
+
+     Variable elt : Type.
+
+     (* Convert a variable map to a variable set. *)
+     Definition vset (m : M.t elt) : VS.t :=
+       fold (fun x _ s => VS.add x s) m VS.empty.
+
+     Lemma mem_vset E :
+       forall x, mem x E -> VS.mem x (vset E).
+     Proof.
+       rewrite /vset.
+       eapply Lemmas.P.fold_rec.
+       - move=> m Hempty x Hmem.
+         apply: False_ind.
+         exact: (Lemmas.empty_mem Hempty Hmem).
+       - move=> x e m E1 E2 _ _ Hadd Hind y Hmem.
+         case Hyx: (y == x).
+         + exact: (VS.Lemmas.mem_add_eq _ Hyx).
+         + move/negP: Hyx => Hyx.
+           rewrite (VS.Lemmas.mem_add_neq _ Hyx).
+           apply: Hind.
+           move: (Hadd y) => {Hadd}.
+           rewrite (VM.Lemmas.find_add_neq _ _ Hyx) => {Hyx} Hfind.
+           rewrite -(VM.Lemmas.find_eq_mem_eq Hfind).
+           exact: Hmem.
+     Qed.
+
+     (* Generate a new variable. *)
+     Definition new_var (m : t elt) : var :=
+       match Lemmas.max_elt m with
+       | Some (v, _) => v + 1
+       | None => 0
+       end.
+
+     Lemma new_var_is_new :
+       forall (m : t elt), ~~ mem (new_var m) m.
+     Proof.
+       move=> m.
+       apply/negP => Hmem.
+       move: (mem_2 Hmem) => {Hmem}.
+       rewrite /new_var.
+       move: (refl_equal (Lemmas.max_elt m)).
+       move: {2}(Lemmas.max_elt m) => x.
+       destruct x.
+       - destruct p as [x ty].
+         move=> Hmax; rewrite Hmax => Hin.
+         move: (Lemmas.max_elt_Above Hmax) => Habove.
+         have: In (x + 1) (remove x m).
+         + case: Hin => ty1 Hmapsto.
+           exists ty1.
+           apply: (remove_2 _ Hmapsto).
+           rewrite addn1 => {Hmax Habove Hmapsto ty ty1 m} Heq.
+           move: (ltnSn x).
+           rewrite {1}(eqP Heq).
+           rewrite ltnn.
+           discriminate.
+         + move=> Hin1.
+           move: (Habove _ Hin1) => Hlt.
+           move: (ltn_trans Hlt (ltnSn x)).
+           rewrite addn1 ltnn.
+           discriminate.
+       - move=> Hmax; rewrite Hmax => Hin.
+         move: (Lemmas.max_elt_Empty Hmax) => Hempty.
+         case: Hin => ty Hmapsto.
+         move: (Hempty 0 ty).
+         apply; assumption.
+     Qed.
+
+   End Aux.
+
+End VM.
